theories/twoLockMSQ_hocap_spec.v
@@ -5,6 +5,7 @@ From iris.heap_lang Require Import lang proofmode notation.
 From iris.heap_lang.lib Require Import lock spin_lock.
 From iris.base_logic.lib Require Import invariants token.
 From MSQueue Require Import MSQ_common.
+From MSQueue Require Import queue_specs.
 From MSQueue Require Import twoLockMSQ_impl.
 
 Local Existing Instance spin_lock.
@@ -46,17 +47,9 @@ Definition TokBefore (g : Qgnames) := token g.(γ_Before).
 Definition TokAfter (g : Qgnames) := token g.(γ_After).
 Definition TokUpdated (g : Qgnames) := ((TokBefore g) ∗ (TokAfter g))%I.
 
-(* ------ Notation for Abstract State of Queue ------ *)
-Notation "Q_γ ⤇● xs_v" := (own Q_γ.(γ_Abst) (●F (to_agree xs_v)))
-  (at level 20, format "Q_γ  ⤇●  xs_v") : bi_scope.
-Notation "Q_γ ⤇◯ xs_v" := (own Q_γ.(γ_Abst) (◯F (to_agree xs_v)))
-  (at level 20, format "Q_γ  ⤇◯  xs_v") : bi_scope.
-Notation "Q_γ ⤇[ q ] xs_v" := (own Q_γ.(γ_Abst) (◯F{ q } (to_agree xs_v)))
-  (at level 20, format "Q_γ  ⤇[ q ]  xs_v") : bi_scope.
-
 (* ----- Queue Invariants ------ *)
 Definition queue_invariant (l_head l_tail : loc) (Q_γ : Qgnames) : iProp Σ :=
-  ∃ xs_v, Q_γ ⤇● xs_v ∗ (* Abstract state *)
+  ∃ xs_v, Q_γ.(γ_Abst) ⤇● xs_v ∗ (* Abstract state *)
   ∃ xs xs_queue xs_old (x_head x_tail: node), (* Concrete state *)
   ⌜xs = xs_queue ++ [x_head] ++ xs_old⌝ ∗
   isLL xs ∗
@@ -97,7 +90,7 @@ Definition queue_invariant (l_head l_tail : loc) (Q_γ : Qgnames) : iProp Σ :=
   ).
 
 Definition queue_invariant_simple (l_head l_tail : loc) (Q_γ : Qgnames) : iProp Σ :=
-  ∃ xs_v, Q_γ ⤇● xs_v ∗ (* Abstract state *)
+  ∃ xs_v, Q_γ.(γ_Abst) ⤇● xs_v ∗ (* Abstract state *)
   ∃ xs xs_queue xs_old (x_head x_tail: node), (* Concrete state *)
   ⌜xs = xs_queue ++ [x_head] ++ xs_old⌝ ∗
   isLL xs ∗
@@ -172,7 +165,7 @@ Proof. apply _. Qed.
 Lemma initialize_spec:
   {{{ True }}}
     initialize #()
-  {{{ v_q Q_γ, RET v_q; is_queue v_q Q_γ ∗ Q_γ ⤇◯ [] }}}.
+  {{{ v_q Q_γ, RET v_q; is_queue v_q Q_γ ∗ Q_γ.(γ_Abst) ⤇◯ [] }}}.
 Proof.
   iIntros (Φ) "_ HΦ".
   wp_lam.
@@ -235,7 +228,7 @@ Qed.
 
 (* ----- Specification for Enqueue ----- *)
 Lemma enqueue_spec v_q (v : val) (Q_γ : Qgnames) (P Q : iProp Σ) :
-  □(∀xs_v, (Q_γ ⤇● xs_v ∗ P ={⊤ ∖ ↑Ni}=∗ ▷ (Q_γ ⤇● (v :: xs_v) ∗ Q))) -∗
+  □(∀xs_v, (Q_γ.(γ_Abst) ⤇● xs_v ∗ P ={⊤ ∖ ↑Ni}=∗ ▷ (Q_γ.(γ_Abst) ⤇● (v :: xs_v) ∗ Q))) -∗
   {{{ is_queue v_q Q_γ ∗ P}}}
     enqueue v_q v
   {{{ w, RET w; Q }}}.
@@ -391,10 +384,10 @@ Qed.
 
 (* ----- Specification for Dequeue ----- *)
 Lemma dequeue_spec v_q (Q_γ : Qgnames) (P : iProp Σ) (Q : val -> iProp Σ):
-  □(∀xs_v, (Q_γ ⤇● xs_v ∗ P
+  □(∀xs_v, (Q_γ.(γ_Abst) ⤇● xs_v ∗ P
               ={⊤ ∖ ↑Ni}=∗
-              ▷ (( ⌜xs_v = []⌝ ∗ Q_γ ⤇● xs_v ∗ Q NONEV) ∨
-              (∃v xs_v', ⌜xs_v = xs_v' ++ [v]⌝ ∗ Q_γ ⤇● xs_v' ∗ Q (SOMEV v)))
+              ▷ (( ⌜xs_v = []⌝ ∗ Q_γ.(γ_Abst) ⤇● xs_v ∗ Q NONEV) ∨
+              (∃v xs_v', ⌜xs_v = xs_v' ++ [v]⌝ ∗ Q_γ.(γ_Abst) ⤇● xs_v' ∗ Q (SOMEV v)))
             )
    )
   -∗
@@ -587,9 +580,12 @@ Qed.
 
 End proofs.
 
-Notation "Q_γ ⤇● xs_v" := (own Q_γ.(γ_Abst) (●F (to_agree xs_v)))
-  (at level 20, format "Q_γ  ⤇●  xs_v") : bi_scope.
-Notation "Q_γ ⤇◯ xs_v" := (own Q_γ.(γ_Abst) (◯F (to_agree xs_v)))
-  (at level 20, format "Q_γ  ⤇◯  xs_v") : bi_scope.
-Notation "Q_γ ⤇[ q ] xs_v" := (own Q_γ.(γ_Abst) (◯F{ q } (to_agree xs_v)))
-  (at level 20, format "Q_γ  ⤇[ q ]  xs_v") : bi_scope.
+(* TODO: figure out what L should be
+Definition twoLockMSQ : queue :=
+{|
+  queue_specs.is_queue Σ _ (_ : ???) _ :=
+    is_queue (nroot.@"two-lock-MSQ");
+  queue_specs.initialize_spec _ _ _ _ := initialize_spec (nroot.@"two-lock-MSQ");
+  queue_specs.enqueue_spec _ _ _ _ := enqueue_spec (nroot.@"two-lock-MSQ");
+  queue_specs.dequeue_spec _ _ _ _ := dequeue_spec (nroot.@"two-lock-MSQ");
+|}. *)
